Common.v
@@ -1,0 +1,35 @@
+(** * Common Definitions *)
+(** Data structures used by other modules. *)
+
+Add LoadPath "/Users/pv/Polya/Coq/pierce_software_foundations_3.2".
+Require Export SfLib.
+Require Import LibTactics.
+
+Module P3Common.
+
+(** ** Association lists (alists) *)
+
+Definition alist (T : Type) : Type := list (id * T).
+
+Fixpoint lookup {X: Type} (x: id) (a: alist X) : option X :=
+  match a with
+    | nil => None
+    | cons (y, v) a' => if eq_id_dec x y then (Some v) else (lookup x a')
+    end.
+
+Lemma lookup_cons_eq : 
+  forall T x (v : T) (a : alist T),
+    lookup x (cons (x, v) a) = Some v.
+Proof.
+  intros. simpl. apply eq_id.
+Qed.
+
+Lemma lookup_cons_neq :
+  forall T x y (v : T) (a : alist T),
+    x <> y ->
+    lookup x (cons (y, v) a) = lookup x a.
+Proof.
+  intros. simpl. apply neq_id. apply H.
+Qed.
+
+End P3Common.
